

Problem Set 4: Discrete Mathematics

Theepakorn Phayenrat 67011352

1. Use the Principle of Mathematical Induction to prove that

$$1 - 2 + 2^2 - 2^3 + \dots + (-1)^n 2^n = \frac{2^{n+1}(-1)^n + 1}{3} \quad \text{for all positive integers } n.$$

2. Use the Principle of Mathematical Induction to prove that $1 + 2^n \leq 3^n$ for all $n \geq 1$.

Problem Set 4: Discrete Mathematics

3. Use the Principle of Mathematical Induction to prove that $1 + 3 + 9 + 27 + \dots + 3^n = \frac{3^{n+1} - 1}{2}$ for all $n \geq 0$.

4. Prove that $\sum_{j=n}^{2n-1} (2j+1) = 3n^2$ for all positive integers n .

Problem Set 4: Discrete Mathematics

5. Prove that for any positive integer n , the number $2^{2^n}-1$ is divisible by 3.

6. Prove that $x^0 + x^1 + \dots + x^n = (x^{n+1}-1)/(x-1)$ for all integers $n \geq 0$, using induction.

Problem Set 4: Discrete Mathematics

7. For each natural number $n \geq 1$, the n^{th} Fibonacci number, F_n , is defined inductively by

$F_1=1$, $F_2 = 1$, and $F_{n+2} = F_{n+1} + F_n$ for $n \geq 1$.

Prove that $F_{n+6} = 4F_{n+3} + F_n$ for $n > 0$.

8. Prove that for any $n \geq 1$, $\sum_{i=1}^n (i^2) = n(n+1)(2n+1)/6$

Problem Set 4: Discrete Mathematics

9. Prove that $n! > 2^n$ for all $n \geq 4$

10. Show that $\sum_{i=1}^n (i^3) = (\sum_{i=1}^n i)^2$ for all $n \geq 1$

1. Use the Principle of Mathematical Induction to prove that

$$1 - 2 + 2^2 - 2^3 + \dots + (-1)^n 2^n = \frac{2^{n+1}(-1)^n + 1}{3} \quad \text{for all positive integers } n.$$

Proof Let $P(n)$ be the statement, " $\forall n \in \mathbb{Z}^+$, $1 - 2 + 2^2 - 2^3 + \dots + (-1)^n 2^n = \frac{2^{n+1}(-1)^n + 1}{3}$ "

We need to show that $P(n)$ is true for all $n \in \mathbb{Z}^+$

Base Case $P(1): 1 - 2^1 = -1$ } True $\therefore \forall n \in \mathbb{Z}^+; 1 - 2 + 2^2 - 2^3 + \dots + (-1)^n 2^n = \frac{(2^{n+1})(-1)^n + 1}{3}$
 $\frac{2^{1+1}(-1)^1 + 1}{3} = \frac{-3}{3} = -1$

is true by Mathematical Induction $\#$

Induction Hypothesis $P(k)$: Assume is true

Induction Step

$$\begin{aligned} P(k) \rightarrow P(k+1): 1 - 2 + 2^2 - 2^3 + \dots + (-1)^{k+1} 2^{k+1} &= 1 - 2 + 2^2 - 2^3 + \dots + (-1)^k 2^k + (-1)^{k+1} 2^{k+1} \\ &= \frac{2^{k+1}(-1)^k + 1}{3} + (-1)^{k+1} 2^{k+1} \\ &= \frac{2^{k+1}(-1)^k + 1}{3} + \frac{3(-1)^{k+1} 2^{k+1}}{3} \\ &= \frac{(2^{k+1}(-1)^k + 1) + 3(-1)^{k+1} 2^{k+1}}{3} \end{aligned}$$

2. Use the Principle of Mathematical Induction to prove that $1 + 2^n \leq 3^n$ for all $n \geq 1$.

Proof $\forall n \in \mathbb{Z}^+; \text{ let } P(n) \text{ be } 1 + 2^n \leq 3^n$

Base Case $P(1): 1 + 2^1 \leq 3^1$
 $3 \leq 3 \leftarrow \text{True}$

Inductive Hypothesis $P(k): 1 + 2^k \leq 3^k$

Inductive Step $P(k) \rightarrow P(k+1): (1 + 2^{k+1}) + 2^k \leq 3^{k+1}$
 $\leq 3^k + 2^k$
 $= 2 \cdot 3^k$
 $< 3 \cdot 3^k$
 $= 3^{k+1} \#$

$\therefore \forall n \in \mathbb{Z}^+; 1 + 2^n \leq 3^n$ is true by Mathematical Induction $\#$

Theepakorn Phayarat 6511352

3. Use the Principle of Mathematical Induction to prove that $1 + 3 + 9 + 27 + \dots + 3^n = \frac{3^{n+1} - 1}{2}$ for all $n \geq 0$.

Proof: Let P_n be

Base Case: $P(0): 1 = \frac{3^{0+1} - 1}{2}$
 $1 = 1 \leftarrow \text{True}$

Induction Hypothesis: $P(k): 1 + 3 + 3^2 + 3^3 + \dots + 3^k = \frac{3^{k+1} - 1}{2}$

Inductive Step: $P(k) \rightarrow P(k+1): 1 + 3 + 3^2 + 3^3 + \dots + 3^{k+1} = 1 + 3 + 3^2 + 3^3 + \dots + 3^k + 3^{k+1} = \frac{3^{k+1} - 1}{2} + 3^{k+1}$

$$= \frac{(3^{k+1} - 1) + 2(3^{k+1})}{2}$$

$$= \frac{3^{k+2} - 1}{2} = \frac{3^{(k+1)+1} - 1}{2}$$

$\therefore 1 + 3 + 9 + 27 + \dots + 3^n = \frac{3^{n+1} - 1}{2}$ is true by Mathematical Induction

4. Prove that $\sum_{j=n}^{2n-1} (2j+1) = 3n^2$ for all positive integers n .

Proof:

Base Case: $P(1): \sum_{j=1}^1 (2j+1) = 3(1)^2$
 $3 = 3 \leftarrow \text{True}$

Induction Hypothesis: $P(k): \sum_{j=k}^{2j-1} (2j+1) = 3(k)^2$

Induction Step: $P(k) \rightarrow P(k+1): \sum_{j=k+1}^{2j-1} (2j+1) = \sum_{j=k}^{2j-1} (2j+1) - (2k+1) + (4k+3)$

$$= 3k^2 - 6k + 3$$

$$= 3(k+1)^2$$

$\therefore \forall n \in \mathbb{Z}^+; \sum_{j=n}^{2j-1} (2j+1) = 3n^2$ is true by Mathematical Induction

Theepakorn Phayantat 67011352

5. Prove that for any positive integer n , the number $2^{2n}-1$ is divisible by 3.

Proof

Let $P(n)$

Base Case

$P(1)$ $2^{2(1)}-1=3(1)$, $1 \in \mathbb{Z}$ which is true.

Induction Hypothesis

Assume $P(k)$: $2^{2k}-1=3(m)$, $m \in \mathbb{Z}$ is true

Induction Step

$P(k) \rightarrow P(k+1)$ $2^{2k+2}-1 = 2^{2k+2}-1$
 $= 2^2(3m+1)-1$
 $= 12m$
 $= 3(4m)$
 $= 3(x)$; $\exists x=4m \in \mathbb{Z}$

$\therefore 3|2^{2n}-1$ *

$\therefore \forall n \in \mathbb{Z}^+$; $3|2^{2n}-1$ by Mathematical Induction *

6. Prove that $x^0+x^1+\dots+x^n = (x^{n+1}-1)/(x-1)$ for all integers $n \geq 0$, using induction.

Proof

$\forall n \in \mathbb{N}$, Let $P(n)$ be " $x^0+x^1+\dots+x^n = \frac{x^{n+1}-1}{x-1}$ "

Base Case

$P(0) = x^0 = \frac{x^{0+1}-1}{x-1}$

$= \frac{x^1-1}{x-1}$

$= 1 = x^0$ which is true *

Induction Hypothesis :

Assume $P(k)$: $x^0+x^1+\dots+x^k = \frac{x^{k+1}-1}{x-1}$; $\forall k \in \mathbb{N}$ is true.

Induction Step :

$P(k) \rightarrow P(k+1)$: $x^0+x^1+\dots+x^k+x^{k+1} = \frac{x^{k+1}-1}{x-1} + x^{k+1}$

$= \frac{(x^{k+1}-1) + (x^{k+1})(x-1)}{x-1}$

$= \frac{(x^{k+1}-1) + (x^{k+2}-x^{k+1})}{x-1}$

$= \frac{x^{k+2}-1}{x-1} = \frac{x^{(k+1)+1}-1}{x-1}$ *

$\therefore \forall n \in \mathbb{N}$; $x^0+x^1+\dots+x^n = \frac{x^{n+1}-1}{x-1}$ is true by Mathematical Induction *

Theopatorn Phayonrat 67011352

7. For each natural number $n \geq 1$, the n^{th} Fibonacci number, F_n , is defined inductively by

$F_1 = 1$, $F_2 = 1$, and $F_{n+2} = F_{n+1} + F_n$ for $n \geq 1$.

Prove that $F_{n+6} = 4F_{n+3} + F_n$ for $n > 0$.

Proof $\forall n \in \mathbb{Z}^+$; Let $P(n)$ be " $F_{n+6} = 4F_{n+3} + F_n$ "

$$F_1 = 1, F_2 = 1, F_3 = 2, F_4 = 3, F_5 = 5, \\ F_6 = 8, F_7 = 13, F_8 = 21, F_9 = 34, F_{10} = 55$$

Base Case

$$P(1): F_{1+6} = F_7 = 13 = 4(F_3) + F_1 \\ = 4(F_3) + F_1 \quad *$$

Induction Hypothesis

Assume that $P(1), P(2), P(3), \dots, P(k)$ are true.

Induction Step

$$P(k) \rightarrow P(k+1): F_{(k+1)+6} = F_{k+7} \\ = F_{k+5} + F_{k+6} \\ = 2F_{k+5} + F_{k+4} \\ = 3F_{k+4} + 2F_{k+3} \\ = F_{k+4} + 4F_{k+3} + 2F_{k+2} \\ = F_{k+4} + (F_{k+6} - F_k) + 2F_{k+2} \\ = F_{k+5} + 2F_{k+4} + 2F_{k+2} - F_k \\ = 3F_{k+4} + F_{k+3} + 2F_{k+2} - F_k \\ = 4F_{k+4} + F_{k+2} - F_k \\ = 4F_{k+4} + F_{k+1} \quad * \\ = 4F_{(k+1)+3} + F_{k+1}$$

" $F_{n+6} = 4F_{n+3} + F_n$ " is true by Strong Mathematical Induction *

8. Prove that for any $n \geq 1$, $\sum_{i=1}^n (i^2) = n(n+1)(2n+1)/6$

Proof $\forall n \in \mathbb{Z}^+$; Let $P(n)$ be " $\sum_{i=1}^n i^2 = \frac{n(n+1)(2n+1)}{6}$ "

Base Case $P(1): 1^2 = 1$ which is true. ✖

Induction Hypothesis: Assume $P(k): 1^2 + 2^2 + 3^2 + \dots + k^2 = \frac{k(k+1)(2k+1)}{6}$ is true.

Induction Step: $P(k) \Rightarrow P(k+1): 1^2 + 2^2 + 3^2 + \dots + k^2 + (k+1)^2 = \frac{k(k+1)(2k+1)}{6} + (k+1)^2$

$$= \frac{[2k^3 + 3k^2 + k] + [6k^2 + 12k + 6]}{6}$$

$$= \frac{2k^3 + 9k^2 + 13k + 6}{6}$$

$$= \frac{(k^2 + 3k + 2)(2k + 3)}{6}$$

$$= \frac{(k+1)[k+1+1][2(k+1)+1]}{6} \quad \#$$

$\therefore \forall n \in \mathbb{Z}^+; \sum_{i=1}^n i^2 = \frac{n(n+1)(2n+1)}{6}$ is true by Mathematical Induction ✖

9. Prove that $n! > 2^n$ for all $n \geq 4$

Proof $\forall n \in \mathbb{Z}^+; \text{ Let } P(n) \text{ be } "n! > 2^n \text{ for all } n \geq 4"$

Base Case $P(4): 4! = 24$
 > 16
 $= 16$ which is true ✖

Induction Hypothesis: Assume $P(k): "k! > 2^k"$ is true.

Induction Step $P(k) \Rightarrow P(k+1): (k+1)! > (k+1)k!$
 $> 2k!$
 $> 2(2^k)$
 $= 2^{k+1} \quad \#$

$\therefore \forall n \in \mathbb{Z}^+; n! > 2^n \text{ for all } n \geq 4$ is true by Mathematical Induction ✖

10. Show that $\sum_{i=1}^n i^3 = \left(\sum_{i=1}^n i\right)^2$ for all $n \geq 1$

Proof $\forall n \in \mathbb{Z}^+$; Let $P(n)$ be $\sum_{i=1}^n i^3 = \left(\sum_{i=1}^n i\right)^2$

Base Case $1^3 = (1^2)^2$ which is true \times

Induction Hypothesis: Assume $P(k)$: $\sum_{i=1}^k i^3 = \left(\sum_{i=1}^k i\right)^2$ is true

Induction Step: $P(k) \rightarrow P(k+1)$: $1^3 + 2^3 + 3^3 + \dots + k^3 + (k+1)^3 = \left(\sum_{i=1}^k i\right)^2 + (k+1)^3$
 $= \left[\frac{k(k+1)}{2}\right]^2 + (k+1)^3$
 $= \frac{k^4 + 2k^3 + k^2 + 4k^3 + 12k^2 + 12k + 4}{4}$
 $= \frac{k^4 + 6k^3 + 13k^2 + 12k + 4}{4}$
 $= \frac{(k+1)^2(k+2)^2}{4}$
 $= \frac{(k+1)^2[(k+1)+1]^2}{2^2}$
 $= \left[\frac{(k+1)[(k+1)+1]}{2}\right]^2 \times$

From 04 DM Induction Very First Pages.

$\therefore \forall n \in \mathbb{Z}^+$; $\sum_{i=1}^n i^3 = \left(\sum_{i=1}^n i\right)^2$ is true by Mathematical Induction \times